src/syntax/FStar.Syntax.Free.fst
@@ -176,8 +176,7 @@ let rec free_names_and_uvs' tm (use_cache:use_cache_t) : free_vars_and_fvars =
 
         | Meta_labeled _
         | Meta_desugared _
-        | Meta_named _
-        | Meta_core_guard -> u1
+        | Meta_named _ -> u1
         end
 
 
