src/syntax/FStar.Syntax.Syntax.fsti
@@ -230,7 +230,6 @@ and metadata =
                                                                  (* Contains the name of the monadic effect and  the type of the subterm *)
   | Meta_monadic_lift  of monad_name * monad_name * typ          (* Sub-effecting: lift the subterm of type typ *)
                                                                  (* from the first monad_name m1 to the second monad name m2 *)
-  | Meta_core_guard                                              (* This term is a guard computed by core checker *)
 and meta_source_info =
   | Sequence                                    (* used when resugaring *)
   | Primop                                      (* ... add more cases here as needed for better code generation *)
